src/EnvI.v
@@ -1,0 +1,62 @@
+Require Import ExtLib.Tactics.Consider.
+Require Import ExtLib.Data.HList.
+Require Import ExtLib.Data.ListNth.
+Require Import ExtLib.Core.Type.
+Require Import MirrorCore.TypesI.
+
+Set Implicit Arguments.
+Set Strict Implicit.
+
+Section Env.
+  Variable typ : Type.
+  Variable typD : list Type -> typ -> Type.
+  Context {RType_typ : RType typD}.
+
+  (** Environments **)
+  Definition tenv : Type := list typ.
+  Definition env : Type := list (sigT (typD nil)).
+  
+  Definition typeof_env (e : env) : tenv :=
+    map (@projT1 _ _) e.
+
+  Definition lookupAs (e : env) (n : nat) (ty : typ) : option (typD nil ty) :=
+    match nth_error e n with
+      | None => None
+      | Some (existT t v) =>
+        match typ_cast (fun x => x) nil t ty with
+          | Some f => Some (f v)
+          | None => None
+        end
+    end.
+
+  Theorem lookupAs_weaken : forall (a b : env) n t x, 
+    lookupAs a n t = Some x ->
+    lookupAs (a ++ b) n t = Some x.
+  Proof.
+    clear. unfold lookupAs. intros.
+    consider (nth_error a n); intros; try congruence.    
+    erewrite nth_error_weaken by eassumption. auto.
+  Qed.
+  
+  Fixpoint split_env (gs : env) : sigT (hlist (typD nil)) :=
+    match gs with
+      | nil => existT _ nil Hnil
+      | g :: gs =>
+        let res := split_env gs in
+        existT _ (projT1 g :: projT1 res) (Hcons (projT2 g) (projT2 res))
+    end.
+
+  Theorem split_env_app : forall gs gs', 
+    split_env (gs ++ gs') = 
+    let (a,b) := split_env gs in
+    let (c,d) := split_env gs' in
+    existT _ (a ++ c) (hlist_app b d).
+  Proof.
+    induction gs; simpl; intros.
+    { destruct (split_env gs'); reflexivity. }
+    { destruct a. rewrite IHgs.
+      destruct (split_env gs).
+      destruct (split_env gs'). reflexivity. }
+  Qed.
+
+End Env.
