src/Ext/Expr.v
@@ -1,8 +1,10 @@
 Require Export Types.
 Require Export ExprCore.
+(*
 Require Export ExprT.
 Require Export ExprFacts.
 Require Export ExprProp.
 Require Export ExprLift.
 Require Export ExprSubst.
 Require Export ExprSimplify.
+*)
